inductive_pointers: Simpler model using classical quotients

theories/lang/cpp/model/inductive_pointers.v
@@ -650,3 +650,433 @@ Module PTRS_IMPL <: PTRS_INTF.
   Include PTRS_DERIVED_MIXIN.
   Include PTRS_MIXIN.
 End PTRS_IMPL.
+
+(* Classical quotients *)
+Parameter quotient : ∀ (A : Set) (R : relation A), Set.
+Infix "/" := quotient.
+Module cquot.
+  Section cquot.
+    Context {A : Set} {R : relation A}.
+
+    Parameter mk : A -> A / R.
+    Parameter lift : ∀ {B} (f : A -> B) (Heq : ∀ x y : A, R x y -> f x = f y), A / R -> B.
+    Axiom ind : ∀ (P : A / R -> Prop),
+      (∀ x : A, P (mk x)) -> (∀ q : A / R, P q).
+
+    Axiom sound : ∀ x y : A, R x y -> mk x = mk y.
+
+    Axiom lift_eq : ∀ {B} {f : A -> B} {Heq x},
+      lift f Heq (mk x) = f x.
+
+    (* Lemma sound_surj : ∀ q : A / R,
+      { a : A | q = mk a }.
+    Proof.
+
+    Definition choose (q : A / R) : A := proj1_sig (sound_surj q).
+    Lemma choose_eq q :
+      q = mk (choose q).
+    Proof. rewrite /choose. by case: sound_surj. Qed.
+    Lemma choose_snd a :
+      R (choose (mk a)) a.
+    Proof. rewrite /choose/=. case: sound_surj =>/=. *)
+
+    #[program] Definition lift2 `{!Reflexive R} {B} (f : A -> A -> B)
+        (Heq : ∀ a11 a12 a21 a22,
+          R a11 a12 -> R a21 a22 -> f a11 a21 = f a12 a22)
+        (q1 q2 : A / R) : B :=
+      cquot.lift (λ ro1, cquot.lift (f ro1) _ q2) _ q1.
+    Next Obligation. intros. exact: Heq. Qed.
+    (* Next Obligation. intros. rewrite /= (choose_eq q2) !lift_eq. exact: Heq. Qed. *)
+    Next Obligation. simpl. intros. induction q2 as [z] using ind. rewrite !lift_eq. exact: Heq. Qed.
+
+    Lemma lift2_eq `{!Reflexive R} {B} (f : A -> A -> B) Heq a1 a2 :
+      cquot.lift2 f Heq (mk a1) (mk a2) = f a1 a2.
+    Proof. by rewrite /lift2 !lift_eq. Qed.
+
+    (* Not very computational; don't care. *)
+    #[global] Declare Instance quot_eq_dec : EqDecision A -> EqDecision (A / R).
+    #[global] Declare Instance quot_countable `{Countable A} : Countable (A / R).
+  End cquot.
+End cquot.
+
+Module PTRS_CLASSIC_IMPL <: PTRS_INTF.
+  (* WIP: alternative, simpler model, using an equivalence relation and classical quotients. *)
+  Module roff_equiv.
+    Inductive roff_equiv : raw_offset -> raw_offset -> Prop :=
+    | o_nil :
+      roff_equiv [] []
+    | o_cons r os1 os2 :
+      roff_equiv os1 os2 ->
+      roff_equiv (r :: os1) (r :: os2)
+    | o_base_derived1 derived base o os1 os2 :
+      roff_equiv os1 os2 ->
+      roff_equiv ((o_base_ derived base, o) :: (o_derived_ base derived, -o) :: os1) os2
+    | o_base_derived2 derived base o os1 os2 :
+      roff_equiv os1 os2 ->
+      roff_equiv os1 ((o_base_ derived base, o) :: (o_derived_ base derived, -o) :: os2)
+    | o_derived_base1 derived base o os1 os2 :
+      roff_equiv os1 os2 ->
+      roff_equiv ((o_derived_ base derived, o) :: (o_base_ derived base, -o) :: os1) os2
+    | o_derived_base2 derived base o os1 os2 :
+      roff_equiv os1 os2 ->
+      roff_equiv os1 ((o_derived_ base derived, o) :: (o_base_ derived base, -o) :: os2)
+    | o_sub_0_equiv1 os1 os2 ty :
+      roff_equiv os1 os2 ->
+      roff_equiv ((o_sub_ ty 0, 0) :: os1) os2
+    | o_sub_0_equiv2 os1 os2 ty :
+      roff_equiv os1 os2 ->
+      roff_equiv os1 ((o_sub_ ty 0, 0) :: os2)
+    | o_sub_sub1 os1 os2 ty z1 z2 o1 o2 :
+      roff_equiv os1 os2 ->
+      roff_equiv ((o_sub_ ty z1, o1) :: (o_sub_ ty z2, o2) :: os1) ((o_sub_ ty (z1 + z2), o1 + o2) :: os2)
+    | o_sub_sub2 os1 os2 ty z1 z2 o1 o2 :
+      roff_equiv os1 os2 ->
+      roff_equiv ((o_sub_ ty (z1 + z2), o1 + o2) :: os1) ((o_sub_ ty z1, o1) :: (o_sub_ ty z2, o2) :: os2)
+    | o_invalid1 os z1 z2 :
+      roff_equiv ((o_invalid_, z1) :: os) [(o_invalid_, z2)]
+    | o_invalid2 os z1 z2 :
+      roff_equiv [(o_invalid_, z1)] ((o_invalid_, z2) :: os)
+    | o_trans os1 os2 os3 :
+      roff_equiv os1 os2 ->
+      roff_equiv os2 os3 ->
+      roff_equiv os1 os3
+    .
+
+    #[local] Hint Constructors roff_equiv : core.
+    #[local] Remove Hints o_trans : core.
+
+    #[local] Instance: Reflexive roff_equiv.
+    Proof. intros ro; induction ro; auto. Qed.
+    #[local] Instance: Transitive roff_equiv.
+    Proof. apply: o_trans. Qed.
+    #[local] Instance: Symmetric roff_equiv.
+    Proof. induction 1; try by constructor. by etrans. Qed.
+    #[export] Instance: Equivalence roff_equiv.
+    Proof. split; apply _. Qed.
+
+    Definition eval_raw_offset (os : raw_offset) : option Z :=
+      foldr (liftM2 Z.add) (Some 0) (eval_offset_seg <$> os).
+
+      (* foldr (Z.add) 0%Z (snd <$> os). *)
+    #[global] Arguments eval_raw_offset !_ /.
+    Lemma eval_raw_offset_proper (x y : raw_offset) :
+      roff_equiv x y → eval_raw_offset x = eval_raw_offset y.
+    Proof.
+      elim => > // _; try lia.
+      all: rewrite /eval_raw_offset ?fmap_cons /= => -> //.
+      all: case: (foldr _ _ _) => //= a; apply (f_equal Some); lia.
+    Qed.
+
+    Lemma roff_equiv_app a11 a12 a21 a22 :
+      roff_equiv a11 a12 ->
+      roff_equiv a21 a22 ->
+      roff_equiv (a21 ++ a11) (a22 ++ a12).
+    Proof.
+      move=> + H. move: a11 a12.
+      induction H => //=; eauto.
+      3: { etrans; first eauto. exact: IHroff_equiv2. }
+      intros. etrans. apply o_invalid1. apply (o_invalid2 _ 0).
+      intros. etrans. apply o_invalid1. apply (o_invalid2 _ 0).
+    Qed.
+  End roff_equiv.
+  Import roff_equiv.
+
+  Definition offset := raw_offset / roff_equiv.
+  #[global] Instance offset_eq_dec : EqDecision offset := _.
+  #[global] Instance offset_countable : Countable offset := _.
+
+  Definition eval_offset' : offset -> option Z :=
+    cquot.lift eval_raw_offset eval_raw_offset_proper.
+  Lemma eval_offset'_eq ro :
+    eval_offset' (cquot.mk ro) = eval_raw_offset ro.
+  Proof. apply cquot.lift_eq. Qed.
+
+  Definition o_id : offset := cquot.mk [].
+  Program Definition mkOffset σ (ro : raw_offset_seg) : offset :=
+    cquot.mk [mk_offset_seg σ ro].
+  Definition o_invalid σ : offset := mkOffset σ o_invalid_.
+  Definition o_field σ f : offset :=
+    mkOffset σ (o_field_ f).
+  Definition o_base σ derived base : offset :=
+    mkOffset σ (o_base_ derived base).
+  Definition o_derived σ base derived : offset :=
+    mkOffset σ (o_derived_ base derived).
+  Program Definition o_sub σ ty z : offset :=
+    mkOffset σ (o_sub_ ty z).
+
+  Inductive base_ptr : Set :=
+  | invalid_ptr_
+  | fun_ptr_ (tu : translation_unit_canon) (o : obj_name)
+  | root (p : root_ptr).
+  #[global] Instance base_ptr_eq_dec : EqDecision base_ptr.
+  Proof. solve_decision. Defined.
+  #[global] Instance root_inj : Inj (=) (=) root.
+  Proof. by intros ?? [=]. Qed.
+
+  Definition ptr : Set := base_ptr * offset.
+  Definition offset_ptr : base_ptr -> offset -> ptr := pair.
+  #[global] Instance ptr_eq_dec : EqDecision ptr.
+  Proof. solve_decision. Defined.
+  #[local] Instance ptr_eq_dec' : EqDecision ptr := ptr_eq_dec.
+  #[global] Declare Instance ptr_countable : Countable ptr.
+  #[global] Instance offset_ptr_inj : Inj2 (=) (=) (=) offset_ptr.
+  Proof. by intros ???? [=]. Qed.
+
+  Definition ptr_alloc_id (p : ptr) : option alloc_id :=
+    match fst p with
+    | invalid_ptr_ => None
+    | fun_ptr_ tu o => Some (global_ptr_encode_aid o)
+    | root p => root_ptr_alloc_id p
+    end.
+
+  Definition base_ptr_vaddr (p : base_ptr) : option vaddr :=
+    match p with
+    | invalid_ptr_ => None
+    | fun_ptr_ tu o => Some (global_ptr_encode_vaddr o)
+    | root p =>
+      root_ptr_vaddr p
+    end.
+
+  Definition ptr_vaddr (p : ptr) : option vaddr :=
+    va ← base_ptr_vaddr (fst p);
+    off ← eval_offset' (snd p);
+    offset_vaddr off va.
+  #[global] Arguments ptr_vaddr !_ /.
+
+  Definition lift_root_ptr (rp : root_ptr) : ptr := (root rp, o_id).
+  #[global] Instance lift_root_ptr_inj : Inj (=) (=) lift_root_ptr.
+  Proof. by intros ?? [=]. Qed.
+  Lemma ptr_vaddr_root_ptr rp :
+    ptr_vaddr (lift_root_ptr rp) = root_ptr_vaddr rp.
+  Proof.
+    rewrite /lift_root_ptr/= eval_offset'_eq.
+    case: root_ptr_vaddr => //= va.
+    by rewrite offset_vaddr_0.
+  Qed.
+
+  Definition invalid_ptr : ptr := (invalid_ptr_, o_id).
+  Definition fun_ptr tu o : ptr := (fun_ptr_ (canonical_tu.tu_to_canon tu) o, o_id).
+
+  Definition null_alloc_id : alloc_id := null_alloc_id.
+  Definition nullptr : ptr := lift_root_ptr nullptr_.
+  Definition global_ptr (tu : translation_unit) o :=
+    lift_root_ptr (global_ptr_ (canonical_tu.tu_to_canon tu) o).
+  Definition alloc_ptr a oid := lift_root_ptr (alloc_ptr_ a oid).
+
+  Lemma global_ptr_nonnull tu o : global_ptr tu o <> nullptr.
+  Proof. done. Qed.
+
+  #[global] Instance global_ptr_inj tu : Inj (=) (=) (global_ptr tu).
+  Proof.
+    rewrite /global_ptr.
+    by intros ?? []%(inj lift_root_ptr)%(inj2 global_ptr_).
+  Qed.
+
+  (* Some proofs using these helpers could be shortened, tactic-wise, but I find
+  them clearer this way, and they work in both models. *)
+  Lemma ptr_vaddr_global_ptr tu o :
+    ptr_vaddr (global_ptr tu o) = Some (global_ptr_encode_vaddr o).
+  Proof. apply ptr_vaddr_root_ptr. Qed.
+  Lemma ptr_alloc_id_global_ptr tu o :
+    ptr_alloc_id (global_ptr tu o) = Some (global_ptr_encode_aid o).
+  Proof. done. Qed.
+
+  Lemma global_ptr_nonnull_addr tu o : ptr_vaddr (global_ptr tu o) <> Some 0%N.
+  Proof. rewrite ptr_vaddr_global_ptr. done. Qed.
+  Lemma global_ptr_nonnull_aid tu o : ptr_alloc_id (global_ptr tu o) <> Some null_alloc_id.
+  Proof. rewrite ptr_alloc_id_global_ptr. done. Qed.
+
+  #[global] Instance global_ptr_addr_inj tu : Inj (=) (=) (λ o, ptr_vaddr (global_ptr tu o)).
+  Proof. intros ??. rewrite !ptr_vaddr_global_ptr. by intros ?%(inj _)%(inj _). Qed.
+  #[global] Instance global_ptr_aid_inj tu : Inj (=) (=) (λ o, ptr_alloc_id (global_ptr tu o)).
+  Proof. intros ??. rewrite !ptr_alloc_id_global_ptr. by intros ?%(inj _)%(inj _). Qed.
+
+  Lemma ptr_vaddr_nullptr : ptr_vaddr nullptr = Some 0%N.
+  Proof. apply ptr_vaddr_root_ptr. Qed.
+
+  Lemma ptr_alloc_id_nullptr : ptr_alloc_id nullptr = Some null_alloc_id.
+  Proof. done. Qed.
+
+  #[program] Definition __o_dot (o1 o2 : offset) : offset :=
+    cquot.lift2 (λ ro1 ro2, cquot.mk (ro2 ++ ro1)) _ o1 o2.
+  Next Obligation. intros; exact /cquot.sound /roff_equiv_app. Qed.
+  Lemma __o_dot_eq (ro1 ro2 : raw_offset) :
+    __o_dot (cquot.mk ro1) (cquot.mk ro2) = cquot.mk (ro2 ++ ro1).
+  Proof. by rewrite /__o_dot cquot.lift2_eq/=. Qed.
+
+  Definition __offset_ptr (p : ptr) (o : offset) : ptr :=
+    (fst p, __o_dot (snd p) o).
+
+  Include PTRS_SYNTAX_MIXIN.
+  (* Duplicated. *)
+  #[global] Notation "p ., o" := (_dot p (o_field _ o))
+    (at level 11, left associativity, only parsing) : stdpp_scope.
+
+  #[local] Ltac UNFOLD_dot := rewrite _dot.unlock/DOT_dot/=.
+  Definition eval_offset σ o := eval_offset' o.
+  Lemma eval_offset_eq σ ro :
+    eval_offset σ (cquot.mk ro) = eval_raw_offset ro.
+  Proof. apply eval_offset'_eq. Qed.
+
+  Lemma foldr_unit {A} (f : A -> A -> A) (z : A) (xs ys : list A) `{!LeftId (=) z f} `{!Assoc (=) f}:
+    fold_right f z (xs ++ ys) =
+    f (fold_right f z xs) (fold_right f z ys).
+  Proof.
+    elim: xs => [//|x xs IH]; cbn. by rewrite {}IH assoc_L.
+  Qed.
+
+  #[global] Instance : Comm (=) add_opt.
+  Proof. move=> [b1|] [b2|] //=. by rewrite comm_L. Qed.
+  #[global] Instance : LeftId (=) (Some 0) add_opt.
+  Proof. by move=> [b1|]. Qed.
+  #[global] Instance : Assoc (=) add_opt.
+  Proof. move=> [b1|] [b2|] [b3|] //=. by rewrite assoc_L. Qed.
+
+  Lemma eval_raw_offset_app ro1 ro2 :
+    eval_raw_offset (ro2 ++ ro1) =
+    add_opt (eval_raw_offset ro1) (eval_raw_offset ro2).
+  Proof. by rewrite (comm_L add_opt) /eval_raw_offset fmap_app foldr_unit. Qed.
+
+  (* [eval_offset] respects the monoidal structure of [offset]s *)
+  Lemma eval_offset_dot σ (o1 o2 : offset) :
+    eval_offset σ (o1 ,, o2) =
+    add_opt (eval_offset σ o1) (eval_offset σ o2).
+  Proof.
+    intros **; UNFOLD_dot.
+    induction o1 as [ro1] using cquot.ind.
+    induction o2 as [ro2] using cquot.ind.
+    by rewrite __o_dot_eq !eval_offset_eq eval_raw_offset_app.
+  Qed.
+
+  #[global] Instance id_dot : LeftId (=) o_id o_dot.
+  Proof.
+    intros o; UNFOLD_dot.
+    induction o as [ro] using cquot.ind.
+    by rewrite __o_dot_eq app_nil_r.
+  Qed.
+
+  Lemma __o_dot_id : RightId (=) o_id __o_dot.
+  Proof.
+    intros o.
+    induction o as [ro] using cquot.ind.
+    by rewrite __o_dot_eq.
+  Qed.
+  #[global] Instance dot_id : RightId (=) o_id o_dot.
+  Proof. UNFOLD_dot. apply __o_dot_id. Qed.
+  #[global] Instance __dot_assoc : Assoc (=) __o_dot.
+  Proof.
+    intros o1 o2 o3.
+    induction o1 as [ro1] using cquot.ind.
+    induction o2 as [ro2] using cquot.ind.
+    induction o3 as [ro3] using cquot.ind.
+    by rewrite !__o_dot_eq assoc_L.
+  Qed.
+
+  #[global] Instance dot_assoc : Assoc (=) o_dot.
+  Proof. UNFOLD_dot. apply _. Qed.
+
+  Implicit Types (p : ptr) (o : offset).
+
+  Lemma offset_ptr_id p : p ,, o_id = p.
+  Proof. UNFOLD_dot. case: p => // p o. by rewrite /__offset_ptr __o_dot_id. Qed.
+
+  Lemma offset_ptr_dot p o1 o2 : p ,, (o1 ,, o2) = p ,, o1 ,, o2.
+  Proof. UNFOLD_dot. by rewrite /__offset_ptr/= assoc_L. Qed.
+
+  Lemma o_sub_0 σ ty :
+    is_Some (size_of σ ty) ->
+    o_sub σ ty 0 = o_id.
+  Proof.
+    intros [n H].
+    apply cquot.sound.
+    rewrite /o_sub /mk_offset_seg/= /o_sub_off/= H /=.
+    exact: roff_equiv.o_sub_0_equiv1.
+  Qed.
+
+  Lemma ptr_alloc_id_offset {p o} :
+    let p' := p ,, o in
+    is_Some (ptr_alloc_id p') -> ptr_alloc_id p' = ptr_alloc_id p.
+  Proof. by UNFOLD_dot. Qed.
+
+  Lemma ptr_vaddr_o_sub_eq p σ ty n1 n2 sz :
+    size_of σ ty = Some sz -> (sz > 0)%N ->
+    same_property ptr_vaddr (p ,, o_sub _ ty n1) (p ,, o_sub _ ty n2) ->
+    n1 = n2.
+  Proof.
+    rewrite same_property_iff.
+    move=> Hsz Hpos [va []]; case: p => [b o].
+    induction o as [os] using cquot.ind.
+    UNFOLD_dot; case: base_ptr_vaddr => //= va'.
+    rewrite !__o_dot_eq /= /o_sub_off Hsz/= !eval_offset'_eq; cbn.
+    destruct (foldr _ _ _) as [Z|] => //=.
+    intros HA%offset_vaddr_inv HB%offset_vaddr_inv; nia.
+  Qed.
+
+  Arguments mk_offset_seg _ !_ /.
+  #[local] Instance: RewriteRelation roff_equiv := {}.
+
+  Lemma o_dot_sub σ (z1 z2 : Z) ty :
+    o_sub σ ty z1 ,, o_sub σ ty z2 = o_sub σ ty (z1 + z2).
+  Proof.
+    rewrite comm_L.
+    UNFOLD_dot; rewrite !__o_dot_eq.
+    apply cquot.sound.
+    rewrite /mk_offset_seg/= /o_sub_off/= /=.
+    destruct size_of => //=; last apply o_invalid1.
+    rewrite roff_equiv.o_sub_sub1; last reflexivity.
+    repeat f_equiv; lia.
+  Qed.
+
+  Lemma _base_derived σ base derived :
+    directly_derives σ derived base ->
+    o_base σ derived base ,, o_derived σ base derived = o_id.
+  Proof.
+    intros [? Hsome].
+    UNFOLD_dot; rewrite !__o_dot_eq /= /o_derived_off /o_base_off Hsome /=.
+    rewrite -{2} (Z.opp_involutive x).
+    exact /cquot.sound /o_derived_base1.
+  Qed.
+
+  Lemma _derived_base σ base derived :
+    directly_derives σ derived base ->
+    o_derived σ base derived ,, o_base σ derived base = o_id.
+  Proof.
+    intros [? Hsome].
+    UNFOLD_dot; rewrite !__o_dot_eq /= /o_derived_off /o_base_off Hsome /=.
+    exact /cquot.sound /o_base_derived1.
+  Qed.
+
+  Lemma o_base_derived σ p base derived :
+    directly_derives σ derived base ->
+    p ,, o_base σ derived base ,, o_derived σ base derived = p.
+  Proof. intros. by rewrite -offset_ptr_dot _base_derived ?offset_ptr_id. Qed.
+
+  Lemma o_derived_base σ p base derived :
+    directly_derives σ derived base ->
+    p ,, o_derived σ base derived ,, o_base σ derived base = p.
+  Proof. intros. by rewrite -offset_ptr_dot _derived_base ?offset_ptr_id. Qed.
+
+  Lemma eval_o_sub σ ty (i : Z) :
+    eval_offset _ (o_sub _ ty i) =
+      (* This order enables reducing for known ty. *)
+      (fun n => Z.of_N n * i) <$> size_of _ ty.
+  Proof.
+    rewrite eval_offset_eq/=/o_sub_off/=.
+    case: size_of=> [sz|] //=.
+    by f_equal; lia.
+  Qed.
+
+  Lemma eval_o_field σ f n cls st :
+    f = {| f_name := n ; f_type := cls |} ->
+    glob_def σ cls = Some (Gstruct st) ->
+    st.(s_layout) = POD \/ st.(s_layout) = Standard ->
+    eval_offset σ (o_field σ f) = offset_of σ (f_type f) (f_name f).
+  Proof.
+    move => -> _ _. cbn.
+    rewrite eval_offset_eq/=/o_field_off/=.
+    case: offset_of => [off|//] /=. by rewrite right_id_L.
+  Qed.
+
+  Include PTRS_DERIVED_MIXIN.
+  Include PTRS_MIXIN.
+End PTRS_CLASSIC_IMPL.
